\documentclass{article}
\usepackage{amsmath}
\usepackage{forest}
\usepackage{tikz} 
\usepackage{tikz-cd} % For diagrams
 \usepackage{quiver}
\usetikzlibrary{automata, positioning, arrows, cd} 

\usepackage{amsthm}
\usepackage{amsfonts}
\usepackage{amsmath}
\usepackage{amssymb}
\usepackage{fullpage}
\usepackage{color}
\usepackage{parskip}
\usepackage{hyperref}
  \hypersetup{
    colorlinks = true,
    urlcolor = blue,       % color of external links using \href
    linkcolor= blue,       % color of internal links 
    citecolor= blue,       % color of links to bibliography
    filecolor= blue,        % color of file links
    }

\usepackage{listings}

\definecolor{dkgreen}{rgb}{0,0.6,0}
\definecolor{gray}{rgb}{0.5,0.5,0.5}
\definecolor{mauve}{rgb}{0.58,0,0.82}

\lstset{frame=tb,
  language=haskell,
  aboveskip=3mm,
  belowskip=3mm,
  showstringspaces=false,
  columns=flexible,
  basicstyle={\small\ttfamily},
  numbers=none,
  numberstyle=\tiny\color{gray},
  keywordstyle=\color{blue},
  commentstyle=\color{dkgreen},
  stringstyle=\color{mauve},
  breaklines=true,
  breakatwhitespace=true,
  tabsize=3,
  escapeinside={(*@}{@*)} % Custom escape settings to handle special chars
}

\newtheoremstyle{theorem}
  {\topsep}   % ABOVESPACE
  {\topsep}   % BELOWSPACE
  {\itshape\/}  % BODYFONT
  {0pt}       % INDENT (empty value is the same as 0pt)
  {\bfseries} % HEADFONT
  {.}         % HEADPUNCT
  {5pt plus 1pt minus 1pt} % HEADSPACE
  {}          % CUSTOM-HEAD-SPEC
\theoremstyle{theorem} 
   \newtheorem{theorem}{Theorem}[section]
   \newtheorem{corollary}[theorem]{Corollary}
   \newtheorem{lemma}[theorem]{Lemma}
   \newtheorem{proposition}[theorem]{Proposition}
\theoremstyle{definition}
   \newtheorem{definition}[theorem]{Definition}
   \newtheorem{example}[theorem]{Example}
\theoremstyle{remark}    
  \newtheorem{remark}[theorem]{Remark}

\title{CPSC-354 Report}
\author{Connor Jacobs \\ Chapman University}

\date{\today} 

\begin{document}

\maketitle

\begin{abstract}
This report will contain a summary of my learning progress throughout the course, so far including: lean proofs
\end{abstract}

\setcounter{tocdepth}{3}
\tableofcontents

\section{Introduction}\label{intro}

This report will document my learning through the course. The content will be structured week by week, with sections on mathematical notes, homework solutions, and personal reflections on the topics discussed.

\section{Week by Week}\label{homework}

\subsection{Week 1}

\subsubsection*{Mathematical Proof}

Proving that $37x + q = 37x + q$ demonstrates the reflexivity property of equality. Reflexivity states that any mathematical expression is equal to itself. In this case, the expression $37x + q$ is compared to itself, and it is immediately clear by the reflexivity of equality that this statement is true.

\subsubsection*{Proof in Lean}

In Lean, the theorem $37x + q = 37x + q$ is proven using the `rfl` tactic. The `rfl` tactic in Lean stands for "reflexivity" and handles proofs of the form $X = X$. When `rfl` is executed, Lean verifies that both sides of the equation are equal and the proof is complete.

The command to execute in Lean is simply:
\begin{verbatim}
rfl
\end{verbatim}

\subsubsection*{Connection Between Lean and Mathematics}

In mathematics, we rely on the axiom of reflexivity to assert that $37x + q = 37x + q$. Likewise, in Lean, the `rfl` tactic automates this process by invoking the same principle. The use of `rfl` in Lean serves as a direct representation of reflexivity in mathematical logic, providing an automated and formalized way to conclude that an expression is equal to itself.

Thus, both in Lean and in traditional mathematics, the proof of $37x + q = 37x + q$ is an application of the same fundamental concept: the reflexivity of equality.

\subsubsection*{Answers to Levels 5-8}

\subsubsection*{Level 5}

\begin{verbatim}
rw [add_zero]
rw [add_zero]
rfl
\end{verbatim}

\subsubsection*{Level 6}

\begin{verbatim}
rw [add_zero c]
rw [add_zero b]
rfl
\end{verbatim}

\subsubsection*{Level 7}

\begin{verbatim}
rw [one_eq_succ_zero]
rw [add_succ]
rw [add_zero]
rfl
\end{verbatim}

\subsubsection*{Level 8}

\begin{verbatim}
rw [two_eq_succ_one]
rw [one_eq_succ_zero]
rw [four_eq_succ_three]
rw [three_eq_succ_two]
rw [two_eq_succ_one]
rw [one_eq_succ_zero]
rw [add_succ]
rw [add_succ]
rw [add_zero]
rfl
\end{verbatim}

\subsection{Week 2}

\subsubsection*{Mathematical Proofs and Lean Implementation}

\textbf{Theorem (Associativity of Addition):} For all natural numbers $a$, $b$, and $c$, the addition operation is associative: $(a + b) + c = a + (b + c)$.

\textit{Proof:} By induction on $c$:

\begin{itemize}
    \item \textbf{Base Case:} When $c = 0$, we have:
    \[
    (a + b) + 0 = a + (b + 0)
    \]
    Using the property addition with zero, this simplifies to:
    \[
    a + b = a + b
    \]
    This equality holds by the reflexivity of equality

    \item \textbf{Inductive Step:} Assume the hypothesis holds for some $d$
    \[
    (a + b) + d = a + (b + d)
    \]
    We must prove $c = \text{succ}(d)$:
    \[
    (a + b) + \text{succ}(d) = a + (b + \text{succ}(d))
    \]
    this can be rewritten as:
    \[
    \text{succ}((a + b) + d) = \text{succ}(a + (b + d))
    \]
    By the inductive hypothesis, we know $(a + b) + d = a + (b + d)$, so:
    \[
    \text{succ}((a + b) + d) = \text{succ}(a + (b + d))
    \]
    This completes the proof of associativity.
\end{itemize}

\textbf{Connection to Lean Proof of Associativity of Addition:}

The Lean proof is the same structure of the mathematical proof:

\begin{verbatim}
induction c with d hd
-- Base case
rw [add_zero]  -- Simplifies (a + b) + 0 to a + b using add_zero
rw [add_zero]  -- Simplifies a + (b + 0) to a + b using add_zero
rfl            -- Reflexivity: confirms a + b = a + b
-- Inductive step
rw [add_succ]  -- Rewrites (a + b) + succ d as succ ((a + b) + d)
rw [hd]        -- Applies the inductive hypothesis: (a + b) + d = a + (b + d)
rw [add_succ]  -- Rewrites a + (b + succ d) as succ (a + (b + d))
rw [add_succ]  -- Confirms that the expressions on both sides match
rfl            -- Reflexivity: confirms succ (a + (b + d)) = succ (a + (b + d))
\end{verbatim}

\textbf{Explanation:}

\begin{itemize}
  \item \textbf{Base Case in Lean:}
  \begin{itemize}
      \item \texttt{rw [add\_zero]} is used twice to simplify both sides of the equation to $a + b$, directly corresponding to the mathematical step where $a + b = a + b$ is shown by reflexivity.
      \item \texttt{rfl} is then used to verify
  \end{itemize}

  \item \textbf{Inductive Step in Lean:}
  \begin{itemize}
      \item \texttt{rw [add\_succ]} rewrites the expression using the definition of addition with the successor, corresponding to the mathematical step where we transition from $(a + b) + \text{succ}(d)$ to $\text{succ}((a + b) + d)$.
      \item \texttt{rw [hd]} applies the inductive hypothesis, mirroring the assumption that $(a + b) + d = a + (b + d)$.
  \end{itemize}
\end{itemize}

\subsubsection*{Week 2 questions}

\textbf{Question:} Can Lean be used to verify complex operations in critical systems such as financial transactions or autonomous vehicles? What are the limitations of its use in such a high stakes environment?

\subsection{Week 3}

\textbf{Discord Name:} connorjacobs

\textbf{Discord Posting:} In my research, I took a look at how advancements in programming languages have balanced performance, safety, and ease of use, focusing on Rust and TypeScript. Rust’s ownership model enforces memory safety by controlling how data is accessed and managed, preventing issues like memory leaks and race conditions without garbage collection. In contrast, TypeScript enhances JavaScript by introducing type checking, catching type errors early, and improving overall code reliability.

\textbf{Link to ReadMe:} \\
\href{https://github.com/Conjac76/WeekThree354/blob/main/README.md}{https://github.com/Conjac76/WeekThree354/blob/main/README.md}

\textbf{Links to two reviews I voted for:} \\
\href{https://github.com/tannerplatt/TannerHW3_354/blob/main/README.md}{https://github.com/tannerplatt/TannerHW3\_354/blob/main/README.md} \\
\href{https://github.com/tyedwards37/Using-LLM-for-Literature-Review}{https://github.com/tyedwards37/Using-LLM-for-Literature-Review}


\subsection{Week 4}

\subsection*{Derivation Trees}

Below are the derivation trees for the given strings using the provided context-free grammar:

\subsubsection*{1. Derivation Tree for \(2+1\)}

\begin{forest}
  [Exp
    [Exp ['2']]
    [\texttt{'+'}]
    [Exp1
      [Exp2 ['1']]
    ]
  ]
\end{forest}

\subsubsection*{2. Derivation Tree for \(1+2*3\)}

\begin{forest}
  [Exp
    [Exp ['1']]
    [\texttt{'+'}]
    [Exp1
      [Exp1 
        [Exp2 ['2']]
      ]
      [\texttt{'*'}]
      [Exp2 ['3']]
    ]
  ]
\end{forest}

\subsubsection*{3. Derivation Tree for \(1+(2*3)\)}

\begin{forest}
  [Exp
    [Exp ['1']]
    [\texttt{'+'}]
    [Exp1
      [Exp2
        [\texttt{'('}]
        [Exp
          [Exp1
            [Exp1
              [Exp2 ['2']]
            ]
            [\texttt{'*'}]
            [Exp2 ['3']]
          ]
        ]
        [\texttt{')'}]
      ]
    ]
  ]
\end{forest}

\subsubsection*{4. Derivation Tree for \((1+2)*3\)}

\begin{forest}
  [Exp
    [Exp1
      [Exp1 
        [Exp2
          [\texttt{'('}]
          [Exp
            [Exp1
              [Exp
                [Exp1
                  [Exp2 ['1']]
                ]
              ]
              [\texttt{'+'}]
              [Exp1
                [Exp2 ['2']]
              ]
            ]
          ]
          [\texttt{')'}]
        ]
      ]
      [\texttt{'*'}]
      [Exp2 ['3']]
    ]
  ]
\end{forest}

\subsubsection*{5. Derivation Tree for \(1+2*3+4*5+6\)}

\begin{forest}
  [Exp
    [Exp
      [Exp 
        [Exp1
          [Exp2 ['1']]
        ]
      ]
      [\texttt{'+'}]
      [Exp1
        [Exp1
          [Exp1 
            [Exp2 ['2']]
          ]
          [\texttt{'*'}]
          [Exp2 ['3']]
        ]
      ]
    ]
    [\texttt{'+'}]
    [Exp1
      [Exp1
        [Exp1 
          [Exp2 ['4']]
        ]
        [\texttt{'*'}]
        [Exp2 ['5']]
      ]
      [\texttt{'+'}]
      [Exp1
        [Exp2 ['6']]
      ]
    ]
  ]
\end{forest}

\subsection{Week 5}

\section*{Solutions to Levels 1-8 (Lean Syntax)}

\subsection*{Level 1}
\texttt{exact todo\_list}

\subsection*{Level 2}
\texttt{exact and\_intro p s}

\subsection*{Level 3}
\texttt{exact and\_intro (and\_intro a i) (and\_intro o u)}

\subsection*{Level 4}
\begin{verbatim}
have p := and_left vm
have p := vm.left
exact p
\end{verbatim}

\subsection*{Level 5}
\texttt{exact h.right}

\subsection*{Level 6}
\texttt{exact and\_intro (and\_left h1) (and\_right h2)}

\subsection*{Level 7}
\begin{verbatim}
have h1 := h.left
have h2 := h1.right
have h3 := h2.left
have h4 := h3.left
have h5 := h4.right
exact h5
\end{verbatim}

\subsection*{Level 8}
\begin{verbatim}
have h1 := h.left
have h2 := h1.left
have h3 := h1.right
have h4 := h.right.right.left
have h5 := h4.left
exact and_intro h3 (and_intro h5 (and_intro h2.left h2.right))
\end{verbatim}

\subsection*{Level 8: Proof in Mathematical Logic}

If $P \land (Q \land R) \land ((S \land T) \land (U \land V))$, then $P \land (S \land U \land V)$.

\begin{align*}
(1) &\quad P \land (Q \land R) \land ((S \land T) \land (U \land V)) \quad & \text{assumption} \\
(2) &\quad P \land (Q \land R) \quad & \text{and\_left (1)} \\
(3) &\quad P \quad & \text{and\_left (2)} \\
(4) &\quad (S \land T) \land (U \land V) \quad & \text{and\_right (1)} \\
(5) &\quad S \land T \quad & \text{and\_left (4)} \\
(6) &\quad U \land V \quad & \text{and\_right (4)} \\
(7) &\quad S \quad & \text{and\_left (5)} \\
(8) &\quad U \quad & \text{and\_left (6)} \\
(9) &\quad V \quad & \text{and\_right (6)} \\
(10) &\quad P \land (S \land U \land V) \quad & \text{and\_intro (3) (7) (8) (9)}
\end{align*}


\subsection{Week 6}


\subsubsection*{Level 1}
\begin{verbatim}
have c : C := bakery_service p
exact c
\end{verbatim}

\subsubsection*{Level 2}
\begin{verbatim}
exact /lambda h : C -> h
\end{verbatim}

\subsubsection*{Level 3}
\begin{verbatim}
exact /lamba h : I ^ S -> ⟨h.right, h.left⟩
\end{verbatim}

\subsubsection*{Level 4}
\begin{verbatim}
exact /lamba c : C -> h2 (h1 c)
\end{verbatim}

\subsubsection*{Level 5}
\begin{verbatim}
have q : Q := h1 p
have t : T := h3 q
have u : U := h5 t
exact u
\end{verbatim}

\subsubsection*{Level 6}
\begin{verbatim}
exact fun c : C => fun d : D => h ⟨c, d⟩
\end{verbatim}

\subsubsection*{Level 7}
\begin{verbatim}
exact fun cd : C ^ D => h cd.left cd.right
\end{verbatim}

\subsubsection*{Level 8}
\begin{verbatim}
exact fun s : S => ⟨h.left s, h.right s⟩
\end{verbatim}

\subsubsection*{Level 9}
\begin{verbatim}
exact fun r : R => ⟨fun s : S => r, fun ns : ¬S => r⟩
\end{verbatim}

\subsubsection*{Question:}
Lambda calculus serves as a foundational framework for computation and formal logic. How can lambda calculus be used to reason about mnore advanced concepts, such as polymorphism?

\subsection{Week 7}

\subsubsection*{Question 1:}

Reduce the following lambda term:
\[ ((\lambda m.\lambda n.m\,n)\,(\lambda f.\lambda x.f\,(f\,x)))\,(\lambda f.\lambda x.f\,(f\,(f\,x))) \]

\textbf{Step 1:}
\begin{align*}
(\lambda m.\lambda n.m\,n)\,(\lambda f.\lambda x.f\,(f\,x)) &\rightarrow \lambda n.(\lambda f.\lambda x.f\,(f\,x))\,n
\end{align*}

\textbf{Step 2:}
\begin{align*}
\lambda n.(\lambda f.\lambda x.f\,(f\,x))\,n\,(\lambda f.\lambda x.f\,(f\,(f\,x))) &\rightarrow (\lambda f.\lambda x.f\,(f\,x))\,(\lambda f.\lambda x.f\,(f\,(f\,x)))
\end{align*}

\textbf{Step 3:} 
\[ \lambda x.((\lambda f.\lambda x.f\,(f\,(f\,x))))\,((\lambda f.\lambda x.f\,(f\,(f\,x)))\,x) \]

\begin{align*}
(\lambda f.\lambda x.f\,(f\,x))\,(\lambda f.\lambda x.f\,(f\,(f\,x))) &\rightarrow \lambda x.[(\lambda f.\lambda x.f\,(f\,(f\,x)))]\,((\lambda f.\lambda x.f\,(f\,(f\,x)))\,x)
\end{align*}

\textbf{Step 4:}
\begin{align*}
(\lambda f.\lambda x.f\,(f\,(f\,x)))\,x &\rightarrow \lambda x.x\,(x\,(x\,x))
\end{align*}

\begin{align*}
(\lambda f.\lambda x.f\,(f\,(f\,x)))\,x &\rightarrow x\,(x\,(x\,x))
\end{align*}

\textbf{Step 5:}
\[ \lambda x.((\lambda f.\lambda x.f\,(f\,(f\,x))))\,(x\,(x\,(x\,x))) \]

\textbf{Step 6:} 
\[ \lambda x.(x\,(x\,(x\,x)))\,(x\,(x\,(x\,x))\,x) \]

\textbf{Step 7:} 
\[ \lambda x.(x\,(x\,(x\,x)))\,(x\,(x\,(x\,x\,x))) \]

the function is applying $x$ six times, which corresponds to the Church numeral 6.


\subsubsection*{Question 2:}

Explain what function on natural numbers $\lambda m.\lambda n.m\,n$ implements.

\subsection*{Answer:}
The lambda term $\lambda m.\lambda n.m\,n$ represents the multiplication operation in Church numerals.

\textbf{Explanation:}
In Church encoding, natural numbers are represented as repeated applications of a function. The numeral $n$ is encoded as $\lambda f.\lambda x.f^n\,x$. The term $m\,n$ applies the function $m$ to $n$. Since $m$ represents applying a function $f$ $m$ times, and $n$ represents applying $f$ $n$ times, their composition results in $m \times n$ applications of $f$. Therefore, $\lambda m.\lambda n.m\,n$ takes two Church numerals and returns their product.

\subsubsection*{Question for Discord:}
Is it possible to represent data structures like pairs or lists using Church numerals and lambda calculus? If so, how do these representations work?

\subsection{Week 8/9}


\textbf{Question 2.}

The expression \texttt{a b c d} reduces to \texttt{(((a b) c) d)} becuase of the way lambda calculus handles application. Application is left associative. The function \texttt{a} is applied to \texttt{b}, then the result is applied to \texttt{c}, and finally, the result is applied to \texttt{d}. This can be written as:

\[
 (((a \, b) \, c) \, d)
\]

\textbf{Question 3.}

In lambda calculus, capture-avoiding substitution prevents bound variable names from unintentionally clashing with free variables. This is implemented in the \texttt{substitute} function, where:

- **Variables**: If a variable matches the name being substituted, it is replaced with the new expression; otherwise, it remains unchanged.

- **Lambda Abstractions**: If the bound variable matches the name being substituted, substitution is skipped for that scope. If not, a fresh name is generated using the \texttt{NameGenerator} to avoid conflicts, and substitution proceeds recursively.

- **Applications**: Substitution occurs recursively in both the function and argument.

\textbf{Example 1 (No Name Conflict)}:
\begin{verbatim}
(\x. \y. x) z
\end{verbatim}
Reduces to: 
\[
\lambda y. z
\]

\textbf{Example 2 (Name Conflict)}:
\begin{verbatim}
(\x. \y. x) y
\end{verbatim}
Reduces to: 
\[
\lambda \text{Var1}. y
\]
where \texttt{Var1} is a fresh variable generated to avoid conflict with \texttt{y}.


\textbf{Question 4.}
No, not all computations in lambda calculus reduce to normal form, and there are situations where evaluation may not terminate or result in a normal form.

Infinite Loops (Divergence): An expression like the following doesn't have a normal form:

\begin{verbatim}
(\x. x x) (\x. x x)
\end{verbatim}

\textbf{Question 5.}
Smallest lambda expression that does not reduce to normal form is known as the Omega combinator

\begin{verbatim}
  (\x. x x) (\x. x x)
\end{verbatim}

\textbf{Question 7.}

\begin{verbatim}
((\m.\n. m n) (\f.\x. f (f x))) (\f.\x. f (f (f x)))
((\Var1. (\f.\x. f (f x)) Var1) ) (\f.\x. f (f (f x)))
(\Var2. (\f.\x. f (f (f x))) ((\f.\x. f (f (f x))) Var2))
\end{verbatim}

\textbf{Question 8.}

\begin{verbatim}
  12: eval (((\m.(\n.(m n))) (\f.(\x.(f (f x))))) (\f.(\x.(f x))))
    39: eval ((\m.(\n.(m n))) (\f.(\x.(f (f x)))))
      39: eval (\m.(\n.(m n)))
      44: substitute ((\n.(m n)), 'm', (\f.(\x.(f (f x)))))
      45: eval (\Var1.((\f.(\x.(f (f x)))) Var1))
    44: substitute (((\f.(\x.(f (f x)))) Var1), 'Var1', (\f.(\x.(f (f (f x))))))
    45: eval ((\Var2.(\Var4.(Var2 (Var2 Var4)))) (\f.(\x.(f (f (f x))))))
      39: eval (\Var2.(\Var4.(Var2 (Var2 Var4))))
      44: substitute ((\Var4.(Var2 (Var2 Var4))), 'Var2', (\f.(\x.(f (f (f x))))))
      45: eval (\Var5.((\f.(\x.(f (f (f x))))) ((\f.(\x.(f (f (f x))))) Var5)))
\end{verbatim}


\textbf{Question on Discord:} -how does left-associative application impact the sequence and structure of reduction steps when evaluating complex expressions

\subsection{Week 10}


\begin{enumerate}
    \item \textbf{Most challenging aspect:} The biggest challenge was managing substitution in a way that avoided unintended variable capture, especially within deeply nested expressions. In the old `evaluate` function, substitution was only partially recursive, which sometimes led to incorrect evaluations when multiple applications or nested abstractions were involved. Ensuring that each function application and lambda abstraction was fully reduced required a more comprehensive approach, where both sides of applications were evaluated recursively and abstractions were reduced in sequence. This transformation was complex but essential for producing a reliable evaluation function.

    \item \textbf{Key insight for Assignment 3:} The key insight emerged from recognizing that the old `evaluate` function only partially evaluated applications by handling a single argument at a time. In the new version, `evaluate` was enhanced to handle both sides of a function application (`app`) recursively, which allowed for a more complete evaluation. Furthermore, an additional case was added to evaluate lambda abstractions (`lam`) by reducing their bodies, creating a more robust and normalized output. This recursive depth and abstraction evaluation were critical in managing nested applications and ensuring proper reduction to normal form.

    \item \textbf{Most interesting takeaway:} One of the most interesting takeaways from this assignment was understanding the full recursive structure required for accurate lambda calculus evaluation.
\end{enumerate}

\noindent \textbf{Question on Discord:} In what ways do modern interpreters and compilers handle complex recursive evaluations to ensure expressions reduce accurately


\subsection{Week 11}

\subsubsection*{Question 1: A = \{\}}

Since the set A is empty, there is nothing to draw for this ARS.

Terminating: Yes 

Confluent: Yes

Unique Normal Forms: Yes

\subsubsection*{Question 2: A = \{a\} and R = \{\}}

\[
\begin{tikzcd}
a
\end{tikzcd}
\]

Terminating: Yes

Confluent: Yes 

Unique Normal Forms: Yes

\subsubsection*{Question 3: A = \{a\} and R = \{a, a\}}

\[
\begin{tikzcd}
a \arrow[loop right]{}
\end{tikzcd}
\]

Terminating: No

Confluent: Yes 

Unique Normal Forms: No

\subsubsection*{Question 4: A = \{a, b, c\} and R = \{(a, b), (a, c)\}}

\[
\begin{tikzcd}
& a \arrow[ld] \arrow[rd] & \\
b & & c
\end{tikzcd}
\]

Terminating: Yes

Confluent: No

Unique Normal Forms: No

\subsubsection*{Question 5: A = \{a, b\} and R = \{(a, a), (a, b)\}}

\[
\begin{tikzcd}
a \arrow[loop above]{} \arrow[r] & b
\end{tikzcd}
\]

Terminating: No

Confluent: Yes

Unique Normal Forms: Yes

\subsubsection*{Question 6: A = \{a, b, c\} and R = \{(a, b), (b, b), (a, c)\}}

\[
\begin{tikzcd}
& a \arrow[ld] \arrow[rd] & \\
b \arrow[loop left]{} & & c
\end{tikzcd}
\]

Terminating: No

Confluent: No

Unique Normal Forms: No

\subsubsection*{Question 7: A = \{a, b, c\} and R = \{(a, b), (b, b), (a, c), (c, c)\}}

\[
\begin{tikzcd}
& a \arrow[ld] \arrow[rd] & \\
b \arrow[loop left]{} & & c \arrow[loop right]{}
\end{tikzcd}
\]

Terminating: No

Confluent: No

Unique Normal Forms: No

\subsubsection*{Homework: Try to find an example of an ARS for each of the possible 8 combinations. Draw pictures of these examples.}

\begin{center}
  \begin{tabular}{|c|c|c|c|c|}
  \hline
  \textbf{Confluent} & \textbf{Terminating} & \textbf{Has UNF} & \textbf{Example} \\
  \hline
  True & True & True & 
  \begin{tikzcd}
  a \arrow[r] & b
  \end{tikzcd} \\
  \hline
  True & True & False & N/A (Impossible) \\
  \hline
  True & False & True & 
  \begin{tikzcd}
  a \arrow[r] & b \arrow[loop right]{}
  \end{tikzcd} \\
  \hline
  True & False & False & 
  \begin{tikzcd}
  a \arrow[loop right]{}
  \end{tikzcd} \\
  \hline
  False & True & True & N/A \\
  \hline
  False & True & False & 
  \begin{tikzcd}
  & a \arrow[ld] \arrow[rd] & \\
  b & & c
  \end{tikzcd} \\
  \hline
  False & False & True & N/A \\
  \hline
  False & False & False & 
  \begin{tikzcd}
  a \arrow[r] & b \arrow[r] & c \arrow[ll, bend left]
  \end{tikzcd} \\
  \hline
  \end{tabular}
  \end{center}

\textbf{Question on Discord:} Why is it impossible to have an ARS that is both Confluent and Terminating but does not have Unique Normal Forms?


\subsection{Week 12} 

\text{Starting Point:}
\[
\text{let rec } \text{fact} = \lambda n. \text{if } n = 0 \text{ then } 1 \text{ else } n \times \text{fact}(n - 1) \text{ in } \text{fact } 3
\]

\text{Step 1: Expanding } \text{let rec}
\[
\text{let } \text{fact} = (\text{fix} \ (\lambda \text{fact}. \lambda n. \text{if } n = 0 \text{ then } 1 \text{ else } n \times \text{fact}(n - 1))) \text{ in } \text{fact } 3
\]

\text{Step 2: Expanding } \text{let}
\[
(\lambda \text{fact}. \text{fact } 3) (\text{fix} \ (\lambda \text{fact}. \lambda n. \text{if } n = 0 \text{ then } 1 \text{ else } n \times \text{fact}(n - 1)))
\]

\text{Step 3: Applying } \text{fix}
\[
(\text{fix} \ (\lambda \text{fact}. \lambda n. \text{if } n = 0 \text{ then } 1 \text{ else } n \times \text{fact}(n - 1))) \ 3
\]
\[
= (\lambda \text{fact}. \lambda n. \text{if } n = 0 \text{ then } 1 \text{ else } n \times \text{fact}(n - 1)) (\text{fix} \ (\lambda \text{fact}. \lambda n. \text{if } n = 0 \text{ then } 1 \text{ else } n \times \text{fact}(n - 1))) \ 3
\]

\text{Step 4: Applying the function}
\[
(\lambda n. \text{if } n = 0 \text{ then } 1 \text{ else } n \times (\text{fix} \ (\lambda \text{fact}. \lambda n. \text{if } n = 0 \text{ then } 1 \text{ else } n \times \text{fact}(n - 1))) (n - 1)) \ 3
\]

\text{Step 5: Computing } \text{if } n = 0
\[
\text{if } 3 = 0 \text{ then } 1 \text{ else } 3 \times (\text{fix} \ (\lambda \text{fact}. \lambda n. \text{if } n = 0 \text{ then } 1 \text{ else } n \times \text{fact}(n - 1))) (3 - 1)
\]
\[
= 3 \times (\text{fix} \ (\lambda \text{fact}. \lambda n. \text{if } n = 0 \text{ then } 1 \text{ else } n \times \text{fact}(n - 1))) \ 2
\]

\text{Step 6: Applying } \text{fix} \text{ again}
\[
3 \times (\lambda \text{fact}. \lambda n. \text{if } n = 0 \text{ then } 1 \text{ else } n \times \text{fact}(n - 1)) (\text{fix} \ (\lambda \text{fact}. \lambda n. \text{if } n = 0 \text{ then } 1 \text{ else } n \times \text{fact}(n - 1))) \ 2
\]

\text{Step 7: Applying the function}
\[
3 \times (\lambda n. \text{if } n = 0 \text{ then } 1 \text{ else } n \times (\text{fix} \ (\lambda \text{fact}. \lambda n. \text{if } n = 0 \text{ then } 1 \text{ else } n \times \text{fact}(n - 1))) (n - 1)) \ 2
\]

\text{Step 8: Computing } \text{if } n = 0 \text{ for } n = 2
\[
3 \times (\text{if } 2 = 0 \text{ then } 1 \text{ else } 2 \times (\text{fix} \ (\lambda \text{fact}. \lambda n. \text{if } n = 0 \text{ then } 1 \text{ else } n \times \text{fact}(n - 1))) (2 - 1))
\]
\[
= 3 \times (2 \times (\text{fix} \ (\lambda \text{fact}. \lambda n. \text{if } n = 0 \text{ then } 1 \text{ else } n \times \text{fact}(n - 1))) \ 1)
\]

\text{Step 9: Applying } \text{fix} \text{ one more time}
\[
3 \times 2 \times (\lambda \text{fact}. \lambda n. \text{if } n = 0 \text{ then } 1 \text{ else } n \times \text{fact}(n - 1)) (\text{fix} \ (\lambda \text{fact}. \lambda n. \text{if } n = 0 \text{ then } 1 \text{ else } n \times \text{fact}(n - 1))) \ 1
\]

\text{Step 10: Applying the function}
\[
3 \times 2 \times (\lambda n. \text{if } n = 0 \text{ then } 1 \text{ else } n \times (\text{fix} \ (\lambda \text{fact}. \lambda n. \text{if } n = 0 \text{ then } 1 \text{ else } n \times \text{fact}(n - 1))) (n - 1)) \ 1
\]

\text{Step 11: Computing } \text{if } n = 0 \text{ for } n = 1
\[
3 \times 2 \times (\text{if } 1 = 0 \text{ then } 1 \text{ else } 1 \times (\text{fix} \ (\lambda \text{fact}. \lambda n. \text{if } n = 0 \text{ then } 1 \text{ else } n \times \text{fact}(n - 1))) (1 - 1))
\]
\[
= 3 \times 2 \times (1 \times (\text{fix} \ (\lambda \text{fact}. \lambda n. \text{if } n = 0 \text{ then } 1 \text{ else } n \times \text{fact}(n - 1))) \ 0)
\]

\text{Step 12: Applying } \text{fix} \text{ again}
\[
3 \times 2 \times 1 \times (\lambda \text{fact}. \lambda n. \text{if } n = 0 \text{ then } 1 \text{ else } n \times \text{fact}(n - 1)) (\text{fix} \ (\lambda \text{fact}. \lambda n. \text{if } n = 0 \text{ then } 1 \text{ else } n \times \text{fact}(n - 1))) \ 0
\]

\text{Step 13: Applying the function}
\[
3 \times 2 \times 1 \times (\lambda n. \text{if } n = 0 \text{ then } 1 \text{ else } n \times (\text{fix} \ (\lambda \text{fact}. \lambda n. \text{if } n = 0 \text{ then } 1 \text{ else } n \times \text{fact}(n - 1))) (n - 1)) \ 0
\]

\text{Step 14: Computing } \text{if } n = 0 \text{ for } n = 0
\[
3 \times 2 \times 1 \times (\text{if } 0 = 0 \text{ then } 1 \text{ else } 0 \times (\text{fix} \ (\lambda \text{fact}. \lambda n. \text{if } n = 0 \text{ then } 1 \text{ else } n \times \text{fact}(n - 1))) (0 - 1))
\]
\[
= 3 \times 2 \times 1 \times 1 \quad (\text{since } 0 = 0, \text{ take the } \text{then} \text{ branch})
\]

\text{Final Computation:}
\[
3 \times 2 \times 1 \times 1 = 6
\]

\text{The result is } 6.

\subsection*{Question for discord:}
are there specific cases where using recursion in lambda calculus can lead to inefficiencies that an iterative approach could solve more cleanly?

  

\section{Lessons from the Assignments}

\subsection{Key Lessons}

The assignments taught the foundational properties in mathematics, such as reflexivity, commutativity, and associativity, and their implementation in Lean. Lean's tactics like `rfl` and `rw` simplify proofs by automating logical steps, making it easier to verify mathematical statements. 

\section{Conclusion}\label{conclusion}

I have learned the connection between mathematical proofs and Lean verification. 

\begin{thebibliography}{99}
\bibitem[BLA], Author, Title, Publisher, Year.
\end{thebibliography}
\end{document}
